WIP class for mayreturn

theories/Basics/MonadPropClosed.v
@@ -1,6 +1,9 @@
 From ExtLib Require Import
      Structures.Monad.
 From ITree Require Import
+     ITree
+     Eq.Eq
+     ITreeMonad
      Basics.Basics
      Basics.Category
      Basics.CategoryKleisli
@@ -11,6 +14,144 @@ From Coq Require Import Morphisms
      Program.Equality.
 
 (* See [PropT.v] in the Vellvm repo for the exact framework to follow with respect to typeclasses, as well as a proof of most monad laws for [PropTM (itree E)] *)
+
+Section MayRet.
+
+  Variable (m: Type -> Type).
+  Context `{Monad m}.
+  Context {EQM : EqM m}.
+
+  (*
+    Given the usual event `Rd (x: loc): E nat`, considering the tree:
+    t == Vis (Rd x) (fun n => ret n)
+    Then with the def from Vellvm specialized to itrees, we have:
+      forall n, MayRet t n
+    While with the following generic definition, to the contrary, we cannot prove `MayRet t n` for any n.
+   *)
+
+  (*
+  Inductive MayRet : forall {A}, m A -> A -> Prop :=
+  | mayret_ret:  forall A (a : A),
+      (* eqm (ret a) b -> *)
+      MayRet (ret a) a
+  | mayret_bind: forall A B (ma: m A) a (k: A -> m B) b,
+      (* eqm c (bind ma k) -> *)
+      MayRet ma a ->
+      MayRet (k a) b ->
+      MayRet (bind ma k) b.
+   *)
+
+
+  Class MayRet: Type :=
+    {
+      mayret: forall {A}, m A -> A -> Prop
+    }.
+
+  Class MayRetCorrect `{MayRet}: Prop :=
+    {
+      mayret_ret_refl : forall {A} (a: A), mayret (ret a) a;
+      mayret_ret_inj  : forall {A} (a a': A), mayret (ret a) a' -> a = a';
+
+      mayret_bind: forall {A B} (ma: m A) (kb: A -> m B) a b,
+          mayret ma a ->
+          mayret (kb a) b ->
+          mayret (bind ma kb) b;
+
+      mayret_bind': forall {A B} (ma: m A) (kb: A -> m B) b,
+          mayret (bind ma kb) b ->
+          exists a, mayret ma a /\ mayret (kb a) b;
+
+      mayret_eqm: forall {A: Type}, Proper (eqm ==> @eq A ==> iff) mayret
+    }.
+
+End MayRet.
+
+Section Instance_MayRet.
+
+  Inductive Returns {E} {A: Type} : itree E A -> A -> Prop :=
+  | ReturnsRet: forall a t, t ≈ Ret a -> Returns t a
+  | ReturnsTau: forall a t, Returns t a -> Returns (Tau t) a
+  | ReturnsVis: forall a {X} (e: E X) (x: X) t k, t ≈ Vis e k -> Returns (k x) a -> Returns t a
+  .
+  Hint Constructors Returns.
+
+  Instance ITree_mayret E: MayRet (itree E) :=
+    {| mayret := @Returns E |}.
+
+  Require Import Paco.paco.
+  Lemma eutt_ret_vis_abs: forall {X Y E} (x: X) (e: E Y) k, Ret x ≈ Vis e k -> False.
+  Proof.
+    intros.
+    punfold H; inv H.
+  Qed.
+
+  Instance Returns_eutt {E A}: Proper (eutt eq ==> @eq A ==> iff) (@Returns E A).
+  Proof.
+    repeat intro; split; intros HRet; subst.
+    - revert y H. induction HRet; intros.
+      constructor; rewrite <- H, H0; reflexivity.
+      apply IHHRet, eqit_inv_tauL; auto.
+      econstructor 3; [rewrite <- H0, H; reflexivity | apply IHHRet; reflexivity].
+    - revert x H; induction HRet; intros ? EQ.
+      constructor; rewrite EQ; eauto.
+      apply IHHRet, eqit_inv_tauR; auto.
+      econstructor 3; [rewrite EQ, H; reflexivity | apply IHHRet; reflexivity].
+  Qed.
+
+  Instance ITree_mayret_correct E: @MayRetCorrect _ _ _ (ITree_mayret E).
+  split.
+  - intros. constructor.
+    reflexivity.
+  - intros. inversion H; subst.
+    + apply eqit_inv_ret in H0; assumption.
+    + apply eutt_ret_vis_abs in H0; contradiction.
+  - induction 1.
+    + intros. rewrite H.
+      cbn. rewrite Eq.bind_ret_l.
+      apply H0.
+    + intros. rewrite tau_eutt.
+      apply IHReturns, H0.
+    + rewrite H. intros.
+      cbn. rewrite bind_vis.
+      eapply (@ReturnsVis _ _ _ _ _ a).
+      reflexivity.
+
+
+
+
+End Instance_MayRet.
+
+
+  (*
+    Goal MayRet t 0.
+    change t with (bind (trigger (Rd x)
+    apply mayret_bind.
+    2: auto.
+    (* MayRet (trigger (Rd x) 0) *)
+
+
+   *)
+
+  Definition ret_f := (fun A (a : A) (ma : m A) => eqm ma (ret a)).
+
+  Lemma ret_f_closed :
+    forall A (a : A), closed_eqm (ret_f A a).
+  Proof.
+    split; intros; unfold ret_f in *;
+      rewrite H0 in *; assumption.
+  Defined.
+
+  Definition bind_f :=
+    fun A B (PA : PropTM A) (K : A -> PropTM B) mb =>
+      exists (ma : m A) (kb : A -> m B),
+        !PA ma /\ (forall a, MayRet ma a -> !(K a) (kb a)) /\
+        Monad.eqm mb (bind ma kb).
+
+
+
+End MayRet.
+
+
 Section Transformer.
 
   Variable (m: Type -> Type).
@@ -40,37 +181,12 @@ Section Transformer.
 
   Global Instance EqM_PropTM : EqM PropTM := eqm2.
 
-  Inductive MayRet : forall {A}, m A -> A -> Prop :=
-  | mayret_ret:  forall A (a : A),
-      (* eqm (ret a) b -> *)
-      MayRet (ret a) a
-  | mayret_bind: forall A B (ma: m A) a (k: A -> m B) b,
-      (* eqm c (bind ma k) -> *)
-      MayRet ma a ->
-      MayRet (k a) b ->
-      MayRet (bind ma k) b.
-
-  Definition ret_f := (fun A (a : A) (ma : m A) => eqm ma (ret a)).
-
-  Lemma ret_f_closed :
-    forall A (a : A), closed_eqm (ret_f A a).
-  Proof.
-    split; intros; unfold ret_f in *;
-      rewrite H0 in *; assumption.
-  Defined.
-
-  Definition bind_f :=
-    fun A B (PA : PropTM A) (K : A -> PropTM B) mb =>
-      exists (ma : m A) (kb : A -> m B),
-        !PA ma /\ (forall a, MayRet ma a -> !(K a) (kb a)) /\
-        Monad.eqm mb (bind ma kb).
-
   (* Let's assume M = id monad
 
 mb = kb ma
 
 fun b =>
-!PA ma K a b
+!PA a /\ K a b
 
  ma: m A ~ ma: A
 kb : A -> m B ~ kb: A -> B
@@ -79,7 +195,7 @@ MayRet ma a ~ a = ma
 
 PA ma /\ (K a mb)
    *)
-  
+
   Lemma bind_f_closed:
     forall A B (PA : PropTM A) (K : A -> PropTM B),
       closed_eqm (bind_f A B PA K).
@@ -131,7 +247,7 @@ Section BAR.
 
   Lemma MayRetret_Eq: forall {A} (a b: A), MayRet (ret a) b -> a = b.
   Proof.
-    intros ? ? ? ?. 
+    intros ? ? ? ?.
     (* inversion H0; subst. *)
     dependent induction H0.
     - apply return_ret_inv.
@@ -144,16 +260,16 @@ Section BAR.
     intros ->.
     - apply return_ret_inv. symmetry; auto.
     - intros ->.
-      apply IHMayRet2. 
-      inversion H0_; subst. 
+      apply IHMayRet2.
+      inversion H0_; subst.
 
       Set Nested Proofs Allowed.
       Lemma ret_eq_bind :
-        forall A B (a: A) (ma: m A) (k : A -> m B), eqm (ret a) (bind ma k) -> 
+        forall A B (a: A) (ma: m A) (k : A -> m B), eqm (ret a) (bind ma k) ->
 
 
-   
-                                    
+
+
 
 
   Lemma ret_bind:
@@ -169,13 +285,13 @@ Section BAR.
       unfold ret_f in Hma. rewrite Hma.
       rewrite bind_ret_l. apply Hk.
       apply mayret_ret. symmetry. apply Hma.
-    - intros Hb. 
+    - intros Hb.
       exists (ret a), (fun x => b'). cbn. repeat split.
       + unfold ret_f. reflexivity.
       + intros a0 Hmr.
         remember (ret a) as ra.
-        revert Heqra. intros. 
-        apply return_ret_inv in H 
+        revert Heqra. intros.
+        apply return_ret_inv in H
         et Nested Proofs Allowed.
         Require Import Coq.Program.Equality.
           (*
@@ -193,5 +309,5 @@ Section BAR.
     unfold Monad_PropTM.
     intro mb. split.
     - intros (ma & kb & HRet & HBind & HEq).
-      rewrite HEq. 
+      rewrite HEq.
 End Transformer.
